libcrux-ml-kem/proofs/fstar/extraction/Libcrux_ml_kem.Ind_cca.Instantiations.Portable.fst
@@ -25,6 +25,15 @@ let validate_private_key
     private_key
     ciphertext
 
+let validate_private_key_only
+      (v_K v_SECRET_KEY_SIZE: usize)
+      (private_key: Libcrux_ml_kem.Types.t_MlKemPrivateKey v_SECRET_KEY_SIZE)
+     =
+  Libcrux_ml_kem.Ind_cca.validate_private_key_only v_K
+    v_SECRET_KEY_SIZE
+    #(Libcrux_ml_kem.Hash_functions.Portable.t_PortableHash v_K)
+    private_key
+
 let decapsulate
       (v_K v_SECRET_KEY_SIZE v_CPA_SECRET_KEY_SIZE v_PUBLIC_KEY_SIZE v_CIPHERTEXT_SIZE v_T_AS_NTT_ENCODED_SIZE v_C1_SIZE v_C2_SIZE v_VECTOR_U_COMPRESSION_FACTOR v_VECTOR_V_COMPRESSION_FACTOR v_C1_BLOCK_SIZE v_ETA1 v_ETA1_RANDOMNESS_SIZE v_ETA2 v_ETA2_RANDOMNESS_SIZE v_IMPLICIT_REJECTION_HASH_INPUT_SIZE:
           usize)
