libcrux-ml-kem/proofs/fstar/extraction/Libcrux_ml_kem.Mlkem768.Avx2.Unpacked.fst
@@ -11,7 +11,49 @@ let _ =
   let open Libcrux_ml_kem.Vector.Traits in
   ()
 
+let key_pair_serialized_private_key
+      (key_pair:
+          Libcrux_ml_kem.Ind_cca.Unpacked.t_MlKemKeyPairUnpacked (sz 3)
+            Libcrux_ml_kem.Vector.Avx2.t_SIMD256Vector)
+     =
+  Libcrux_ml_kem.Ind_cca.Unpacked.impl_4__serialized_private_key (sz 3)
+    #Libcrux_ml_kem.Vector.Avx2.t_SIMD256Vector
+    (sz 1152)
+    (sz 2400)
+    (sz 1184)
+    (sz 1152)
+    key_pair
+
+let key_pair_serialized_private_key_mut
+      (key_pair:
+          Libcrux_ml_kem.Ind_cca.Unpacked.t_MlKemKeyPairUnpacked (sz 3)
+            Libcrux_ml_kem.Vector.Avx2.t_SIMD256Vector)
+      (serialized: Libcrux_ml_kem.Types.t_MlKemPrivateKey (sz 2400))
+     =
+  let serialized:Libcrux_ml_kem.Types.t_MlKemPrivateKey (sz 2400) =
+    Libcrux_ml_kem.Ind_cca.Unpacked.impl_4__serialized_private_key_mut (sz 3)
+      #Libcrux_ml_kem.Vector.Avx2.t_SIMD256Vector
+      (sz 1152)
+      (sz 2400)
+      (sz 1184)
+      (sz 1152)
+      key_pair
+      serialized
+  in
+  serialized
+
 let key_pair_serialized_public_key
+      (key_pair:
+          Libcrux_ml_kem.Ind_cca.Unpacked.t_MlKemKeyPairUnpacked (sz 3)
+            Libcrux_ml_kem.Vector.Avx2.t_SIMD256Vector)
+     =
+  Libcrux_ml_kem.Ind_cca.Unpacked.impl_4__serialized_public_key (sz 3)
+    #Libcrux_ml_kem.Vector.Avx2.t_SIMD256Vector
+    (sz 1152)
+    (sz 1184)
+    key_pair
+
+let key_pair_serialized_public_key_mut
       (key_pair:
           Libcrux_ml_kem.Ind_cca.Unpacked.t_MlKemKeyPairUnpacked (sz 3)
             Libcrux_ml_kem.Vector.Avx2.t_SIMD256Vector)
@@ -34,7 +76,7 @@ let serialized_public_key
       (serialized: Libcrux_ml_kem.Types.t_MlKemPublicKey (sz 1184))
      =
   let serialized:Libcrux_ml_kem.Types.t_MlKemPublicKey (sz 1184) =
-    Libcrux_ml_kem.Ind_cca.Unpacked.impl_3__serialized_public_key_mut (sz 3)
+    Libcrux_ml_kem.Ind_cca.Unpacked.impl_3__serialized_mut (sz 3)
       #Libcrux_ml_kem.Vector.Avx2.t_SIMD256Vector
       (sz 1152)
       (sz 1184)
@@ -63,7 +105,7 @@ let encapsulate
     (sz 1152) (sz 960) (sz 128) (sz 10) (sz 4) (sz 320) (sz 2) (sz 128) (sz 2) (sz 128) public_key
     randomness
 
-let generate_key_pair
+let generate_key_pair_mut
       (randomness: t_Array u8 (sz 64))
       (key_pair:
           Libcrux_ml_kem.Ind_cca.Unpacked.t_MlKemKeyPairUnpacked (sz 3)
@@ -83,6 +125,20 @@ let generate_key_pair
   in
   key_pair
 
+let generate_key_pair (randomness: t_Array u8 (sz 64)) =
+  let key_pair:Libcrux_ml_kem.Ind_cca.Unpacked.t_MlKemKeyPairUnpacked (sz 3)
+    Libcrux_ml_kem.Vector.Avx2.t_SIMD256Vector =
+    Core.Default.f_default #(Libcrux_ml_kem.Ind_cca.Unpacked.t_MlKemKeyPairUnpacked (sz 3)
+          Libcrux_ml_kem.Vector.Avx2.t_SIMD256Vector)
+      #FStar.Tactics.Typeclasses.solve
+      ()
+  in
+  let key_pair:Libcrux_ml_kem.Ind_cca.Unpacked.t_MlKemKeyPairUnpacked (sz 3)
+    Libcrux_ml_kem.Vector.Avx2.t_SIMD256Vector =
+    generate_key_pair_mut randomness key_pair
+  in
+  key_pair
+
 let init_key_pair (_: Prims.unit) =
   Core.Default.f_default #(Libcrux_ml_kem.Ind_cca.Unpacked.t_MlKemKeyPairUnpacked (sz 3)
         Libcrux_ml_kem.Vector.Avx2.t_SIMD256Vector)
@@ -94,6 +150,25 @@ let init_public_key (_: Prims.unit) =
         Libcrux_ml_kem.Vector.Avx2.t_SIMD256Vector)
     #FStar.Tactics.Typeclasses.solve
     ()
+
+let key_pair_from_private_mut
+      (private_key: Libcrux_ml_kem.Types.t_MlKemPrivateKey (sz 2400))
+      (key_pair:
+          Libcrux_ml_kem.Ind_cca.Unpacked.t_MlKemKeyPairUnpacked (sz 3)
+            Libcrux_ml_kem.Vector.Avx2.t_SIMD256Vector)
+     =
+  let key_pair:Libcrux_ml_kem.Ind_cca.Unpacked.t_MlKemKeyPairUnpacked (sz 3)
+    Libcrux_ml_kem.Vector.Avx2.t_SIMD256Vector =
+    Libcrux_ml_kem.Ind_cca.Instantiations.Avx2.Unpacked.keypair_from_private_key (sz 3)
+      (sz 2400)
+      (sz 1152)
+      (sz 1184)
+      (sz 1152)
+      (sz 1152)
+      private_key
+      key_pair
+  in
+  key_pair
 
 let public_key
       (key_pair:
