libcrux-ml-kem/proofs/fstar/extraction/Libcrux_ml_kem.Ind_cca.Instantiations.Avx2.fsti
@@ -33,6 +33,12 @@ val validate_private_key
         v_CIPHERTEXT_SIZE == Spec.MLKEM.v_CPA_CIPHERTEXT_SIZE v_K)
       (fun _ -> Prims.l_True)
 
+/// Private key validation
+val validate_private_key_only
+      (v_K v_SECRET_KEY_SIZE: usize)
+      (private_key: Libcrux_ml_kem.Types.t_MlKemPrivateKey v_SECRET_KEY_SIZE)
+    : Prims.Pure bool Prims.l_True (fun _ -> Prims.l_True)
+
 val decapsulate_avx2
       (v_K v_SECRET_KEY_SIZE v_CPA_SECRET_KEY_SIZE v_PUBLIC_KEY_SIZE v_CIPHERTEXT_SIZE v_T_AS_NTT_ENCODED_SIZE v_C1_SIZE v_C2_SIZE v_VECTOR_U_COMPRESSION_FACTOR v_VECTOR_V_COMPRESSION_FACTOR v_C1_BLOCK_SIZE v_ETA1 v_ETA1_RANDOMNESS_SIZE v_ETA2 v_ETA2_RANDOMNESS_SIZE v_IMPLICIT_REJECTION_HASH_INPUT_SIZE:
           usize)
