libcrux-ml-kem/proofs/fstar/extraction/Libcrux_ml_kem.Ind_cca.Instantiations.Portable.Unpacked.fsti
@@ -80,6 +80,20 @@ val generate_keypair
         v_ETA1_RANDOMNESS_SIZE == Spec.MLKEM.v_ETA1_RANDOMNESS_SIZE v_K)
       (fun _ -> Prims.l_True)
 
+/// Take a serialized private key and generate an unpacked key pair from it.
+val keypair_from_private_key
+      (v_K v_SECRET_KEY_SIZE v_CPA_SECRET_KEY_SIZE v_PUBLIC_KEY_SIZE v_BYTES_PER_RING_ELEMENT v_T_AS_NTT_ENCODED_SIZE:
+          usize)
+      (private_key: Libcrux_ml_kem.Types.t_MlKemPrivateKey v_SECRET_KEY_SIZE)
+      (key_pair:
+          Libcrux_ml_kem.Ind_cca.Unpacked.t_MlKemKeyPairUnpacked v_K
+            Libcrux_ml_kem.Vector.Portable.Vector_type.t_PortableVector)
+    : Prims.Pure
+      (Libcrux_ml_kem.Ind_cca.Unpacked.t_MlKemKeyPairUnpacked v_K
+          Libcrux_ml_kem.Vector.Portable.Vector_type.t_PortableVector)
+      Prims.l_True
+      (fun _ -> Prims.l_True)
+
 /// Get the unpacked public key.
 val unpack_public_key
       (v_K v_T_AS_NTT_ENCODED_SIZE v_RANKED_BYTES_PER_RING_ELEMENT v_PUBLIC_KEY_SIZE: usize)
