libcrux-ml-kem/proofs/fstar/extraction/Libcrux_ml_kem.Ind_cca.Instantiations.Portable.fsti
@@ -13,7 +13,7 @@ let _ =
   let open Libcrux_ml_kem.Vector.Traits in
   ()
 
-/// Portable private key validation
+/// Private key validation
 val validate_private_key
       (v_K v_SECRET_KEY_SIZE v_CIPHERTEXT_SIZE: usize)
       (private_key: Libcrux_ml_kem.Types.t_MlKemPrivateKey v_SECRET_KEY_SIZE)
@@ -23,6 +23,12 @@ val validate_private_key
         Spec.MLKEM.is_rank v_K /\ v_SECRET_KEY_SIZE == Spec.MLKEM.v_CCA_PRIVATE_KEY_SIZE v_K /\
         v_CIPHERTEXT_SIZE == Spec.MLKEM.v_CPA_CIPHERTEXT_SIZE v_K)
       (fun _ -> Prims.l_True)
+
+/// Private key validation
+val validate_private_key_only
+      (v_K v_SECRET_KEY_SIZE: usize)
+      (private_key: Libcrux_ml_kem.Types.t_MlKemPrivateKey v_SECRET_KEY_SIZE)
+    : Prims.Pure bool Prims.l_True (fun _ -> Prims.l_True)
 
 /// Portable decapsulate
 val decapsulate
@@ -81,7 +87,7 @@ val generate_keypair
         v_ETA1_RANDOMNESS_SIZE == Spec.MLKEM.v_ETA1_RANDOMNESS_SIZE v_K)
       (fun _ -> Prims.l_True)
 
-/// Portable public key validation
+/// Public key validation
 val validate_public_key
       (v_K v_RANKED_BYTES_PER_RING_ELEMENT v_PUBLIC_KEY_SIZE: usize)
       (public_key: t_Array u8 v_PUBLIC_KEY_SIZE)
