libcrux-ml-kem/proofs/fstar/extraction/Libcrux_ml_kem.Mlkem768.Neon.Unpacked.fsti
@@ -12,12 +12,30 @@ let _ =
   let open Libcrux_ml_kem.Vector.Traits in
   ()
 
+/// Get the serialized private key.
+val key_pair_serialized_private_key
+      (key_pair:
+          Libcrux_ml_kem.Ind_cca.Unpacked.t_MlKemKeyPairUnpacked (sz 3)
+            Libcrux_ml_kem.Vector.Neon.Vector_type.t_SIMD128Vector)
+    : Prims.Pure (Libcrux_ml_kem.Types.t_MlKemPrivateKey (sz 2400))
+      Prims.l_True
+      (fun _ -> Prims.l_True)
+
+/// Get the serialized private key.
+val key_pair_serialized_private_key_mut
+      (key_pair:
+          Libcrux_ml_kem.Ind_cca.Unpacked.t_MlKemKeyPairUnpacked (sz 3)
+            Libcrux_ml_kem.Vector.Neon.Vector_type.t_SIMD128Vector)
+      (serialized: Libcrux_ml_kem.Types.t_MlKemPrivateKey (sz 2400))
+    : Prims.Pure (Libcrux_ml_kem.Types.t_MlKemPrivateKey (sz 2400))
+      Prims.l_True
+      (fun _ -> Prims.l_True)
+
 /// Get the serialized public key.
 val key_pair_serialized_public_key
       (key_pair:
           Libcrux_ml_kem.Ind_cca.Unpacked.t_MlKemKeyPairUnpacked (sz 3)
             Libcrux_ml_kem.Vector.Neon.Vector_type.t_SIMD128Vector)
-      (serialized: Libcrux_ml_kem.Types.t_MlKemPublicKey (sz 1184))
     : Prims.Pure (Libcrux_ml_kem.Types.t_MlKemPublicKey (sz 1184))
       (requires
         forall (i: nat).
@@ -26,6 +44,16 @@ val key_pair_serialized_public_key
                   .f_ind_cpa_public_key
                   .f_t_as_ntt
                 i))
+      (fun _ -> Prims.l_True)
+
+/// Get the serialized public key.
+val key_pair_serialized_public_key_mut
+      (key_pair:
+          Libcrux_ml_kem.Ind_cca.Unpacked.t_MlKemKeyPairUnpacked (sz 3)
+            Libcrux_ml_kem.Vector.Neon.Vector_type.t_SIMD128Vector)
+      (serialized: Libcrux_ml_kem.Types.t_MlKemPublicKey (sz 1184))
+    : Prims.Pure (Libcrux_ml_kem.Types.t_MlKemPublicKey (sz 1184))
+      Prims.l_True
       (fun _ -> Prims.l_True)
 
 /// Get the serialized public key.
@@ -76,11 +104,19 @@ val encapsulate
       (fun _ -> Prims.l_True)
 
 /// Generate ML-KEM 768 Key Pair in "unpacked" form.
-val generate_key_pair
+val generate_key_pair_mut
       (randomness: t_Array u8 (sz 64))
       (key_pair:
           Libcrux_ml_kem.Ind_cca.Unpacked.t_MlKemKeyPairUnpacked (sz 3)
             Libcrux_ml_kem.Vector.Neon.Vector_type.t_SIMD128Vector)
+    : Prims.Pure
+      (Libcrux_ml_kem.Ind_cca.Unpacked.t_MlKemKeyPairUnpacked (sz 3)
+          Libcrux_ml_kem.Vector.Neon.Vector_type.t_SIMD128Vector)
+      Prims.l_True
+      (fun _ -> Prims.l_True)
+
+/// Generate ML-KEM 768 Key Pair in "unpacked" form.
+val generate_key_pair (randomness: t_Array u8 (sz 64))
     : Prims.Pure
       (Libcrux_ml_kem.Ind_cca.Unpacked.t_MlKemKeyPairUnpacked (sz 3)
           Libcrux_ml_kem.Vector.Neon.Vector_type.t_SIMD128Vector)
@@ -99,6 +135,18 @@ val init_key_pair: Prims.unit
 val init_public_key: Prims.unit
   -> Prims.Pure
       (Libcrux_ml_kem.Ind_cca.Unpacked.t_MlKemPublicKeyUnpacked (sz 3)
+          Libcrux_ml_kem.Vector.Neon.Vector_type.t_SIMD128Vector)
+      Prims.l_True
+      (fun _ -> Prims.l_True)
+
+/// Get an unpacked key from a private key.
+val key_pair_from_private_mut
+      (private_key: Libcrux_ml_kem.Types.t_MlKemPrivateKey (sz 2400))
+      (key_pair:
+          Libcrux_ml_kem.Ind_cca.Unpacked.t_MlKemKeyPairUnpacked (sz 3)
+            Libcrux_ml_kem.Vector.Neon.Vector_type.t_SIMD128Vector)
+    : Prims.Pure
+      (Libcrux_ml_kem.Ind_cca.Unpacked.t_MlKemKeyPairUnpacked (sz 3)
           Libcrux_ml_kem.Vector.Neon.Vector_type.t_SIMD128Vector)
       Prims.l_True
       (fun _ -> Prims.l_True)
